Let us apply the Benders decomposition to the following nonlinear problem:

\[
\begin{array}{rl}
\min& c^{\top}x+f(y)\\
\mathrm{s.t.}& Ax+g(y)\geq b\\
& x\geq 0\\
& y\in\mathbb{Y}
\end{array}
\tag{1}
\]

We define an auxiliary function $h\colon\mathbb{Y}\to\mathbb{R}$ as
 
\[
\begin{array}{c}
h(y)=\min\{c^{\top}x\colon Ax\geq b-g(y),x\geq0\}=\\
\max\{\bigl(b-g(y)\bigr)^{\top}z\colon A^{\top}z\leq c,z\geq 0\}.
\end{array}
\]

Then problem (1) is equivalent to the following problem

\[
\begin{array}{rl}
\min& f(y)+h(y)\\
\mathrm{s.t.}& y\in\mathbb{Y}
\end{array}
\tag{2}
\]

Denote $P=\{z\colon A^{\top}z\leq c,z\geq 0\}$. According to the 
[decomposition theorem](23_12_07_12_27.md), $P=Q+C$ where 
$Q=\mathrm{hull}\{z_{1},z_{2},\ldots,z_{s}\}$ is a polytope and
$C=\mathrm{cone}\{v_{1},v_{2},\ldots,v_{t}\}$ is a finitely generated cone.
Then problem (2) is equivalent to the following problem

\[
\begin{array}{rl}
\min& f(y)+h\\
\mathrm{s.t.}& \bigl(b-g(y)\bigr)^{\top}z_{i}\leq h,\;1\leq i\leq s\\
& \bigl(b-g(y)\bigr)^{\top}v_{j}\leq 0,\;1\leq j\leq t\\
& h\in\mathbb{R}\\
&y\in\mathbb{Y}
\end{array}
\tag{3}
\]

Usually there are a lot of $z_{i}$ and $v_{j}$, so formulation (3) is 
impractical. Applying the Benders decomposition, we start from the problem

\[
\begin{array}{rl}
\min& f(y)+h\\
\mathrm{s.t.}& h\in\mathbb{R}\\
&y\in\mathbb{Y}
\end{array}
\tag{4}
\]

Let $(y^{\star},h^{\star})$ be a solution of problem (4). Then we consider the 
following problem

\[
\begin{array}{rl}
\max& \bigl(b-g(y^{\star})\bigr)^{\top}z\\
\mathrm{s.t.}& A^{\top}z\leq c\\
&z\geq 0
\end{array}
\tag{5}
\]

If problem (5) is unbounded, then there is $v_{j}$ such
that $\bigl(b-g(y^{\star})\bigr)^{\top}v_{j}> 0$. We add a new constraint
$\bigl(b-g(y)\bigr)^{\top}v_{j}\leq 0$ to problem (4).  

If problem (5) has an optimal solution $z_{i}$, then we have two cases:

1. If $h^{\star}=\bigl(b-g(y^{\star})\bigr)^{\top}z_{i}$, then $(x^{\star},y^{\star})$ is an 
optimal solution of problem (1) where 
$x^{\star}=\mathrm{argmin}\{c^{\top}x\colon Ax\geq b-g(y^{\star}), x\geq 0\}$. 

2. If $h^{\star}<\bigl(b-g(y^{\star})\bigr)^{\top}z_{i}$, then we add 
a new constraint $\bigl(b-g(y)\bigr)^{\top}z_{i}\leq h$ to problem (4).

If we have not yet received a solution of problem (1), then we solve the 
updated problem (4) and repeat the steps described above.