Given a system of linear inequalities 

\[
Ax\leq b
\tag{1}
\]

where $A=(a_{ij})_{i,j=1}^{n,m}\in\mathbb{R}^{n\times m}$ and 
$b=(b_{i})_{i=1}^{n}\in\mathbb{R}^{n}$. Let us eliminate $x_{1}$ from 
system (1). To do this, we modify each inequality 

\[
a_{i1}x_{1}+a_{i2}x_{2}+ \ldots+a_{im}x_{m}\leq 0
\]

depending on the sign of $a_{i1}$:

1. $x_{1}+\sum\limits_{j=2}^{m}\dfrac{a_{ij}}{a_{i1}}x_{j}\leq 
    \dfrac{b_{i}}{a_{i1}}$ if $a_{i1}>0$;
2. $-x_{1}+\sum\limits_{j=2}^{m}\dfrac{a_{ij}}{-a_{i1}}x_{j}\leq 
    \dfrac{b_{i}}{-a_{i1}}$ if $a_{i1}<0$;
3. $\sum\limits_{j=2}^{m}a_{ij}x_{j}\leq b_{i}$ if $a_{i1}=0$.

Denote $\bar{x}=(x_{2},x_{3},\ldots,x_{m})^{\top}$. Simplifying the notation, 
we write every inequality of the first type as 
$x_{1}+\bar{a}_{i_{1}}^{\top}\bar{x}\leq\bar{b}_{i_{1}}$, 
every inequality of the second type as 
$-x_{1}+\bar{a}_{i_{2}}^{\top}\bar{x}\leq\bar{b}_{i_{2}}$, 
and every inequality of the third type as 
$\bar{a}_{i_{3}}^{\top}\bar{x}\leq\bar{b}_{i_{3}}$.

Now we compose a new system with fewer number of variables $x_{2}$, $x_{3}$,
 $\ldots$, $x_{m}$. This system consists of inequalities of the third type
 and all possible sums of inequalities of the first and second types:

\[
\begin{cases}
\bar{a}_{i_{3}}^{\top}\bar{x}\leq\bar{b}_{i_{3}},\\
(\bar{a}_{i_{1}}+\bar{a}_{i_{2}})^{\top}\bar{x}\leq\bar{b}_{i_{1}}+\bar{b}_{i_{2}}.
\end{cases}
\tag{2}
\]

<div class="block-head">Theorem</div>
<div class="block-body">
System (1) has a solution if and only if system (2) has a solution. 
</div>

$\rhd$ One part of the statement is obvious. Indeed, if system (1) has a 
solution $x=(x_{1},x_{2},\ldots,x_{m})^{\top}$, then $\bar{x}=(x_{2},x_{3},
\ldots,x_{m})^{\top}$ is a solution of system (2). 

Now, let $\bar{x}=(x_{2},x_{3},\ldots,x_{m})^{\top}$ be a solution of 
system (2). We have

\[
\bar{a}_{i_{2}}^{\top}\bar{x}-\bar{b}_{i_{2}}\leq \bar{b}_{i_{1}}-\bar{a}_{i_{1}}^{\top}\bar{x}.
\]

Therefore, to construct a solution of system (1) we can just take an arbitrary

\[
x_{1}\in[\max\limits_{i_{2}}(\bar{a}_{i_{2}}^{\top}\bar{x}-\bar{b}_{i_{2}}),
\min\limits_{i_{1}}(\bar{b}_{i_{1}}-\bar{a}_{i_{1}}^{\top}\bar{x})].\quad\lhd
\]

The described above variable elimination method is called 
*Fourier-Motzkin Elimination*.